\item Given
  \begin{equation}
    A = \begin{bmatrix}
-5 & -6 & 0\\
2 & 2 & 0\\
0 & 0 & -3
\end{bmatrix}
\end{equation}
  \begin{enumerate}
  \item Find $A^{-1}$ using the Cayley-Hamilton theorem \\
    \begin{itemize}
    \item solve for eigenvalues \\
      \begin{equation}
        \Delta(\lambda) = (\lambda I - A) = 0
      \end{equation}
      \begin{equation}
        \lambda = -1, -2, -3
      \end{equation}
    \item solve for $\beta_0$, $\beta_1$ $\beta_2$\\
      \begin{equation}
        f(\lambda) = \beta_0 + \beta_1\lambda + \beta_2\lambda^2
      \end{equation}
      \begin{equation}
        -1 = \beta_0 - \beta_1 + \beta_2
      \end{equation}
      \begin{equation}
        -\frac 1 2 = \beta_0 - 2\beta_1 + 4\beta_2
      \end{equation}
      \begin{equation}
        -\frac 1 3 = \beta_0 - 3\beta_1 + 9\beta_2
      \end{equation}
      \begin{equation}
        \begin{bmatrix}
          1 & -1 & 1 \\
          1 & -2 & 4 \\
          1 & -3 & 9
        \end{bmatrix}^{-1}
        \begin{bmatrix}
          -1 \\
          -\frac 1 2 \\
          -\frac 1 3
        \end{bmatrix} =
        \begin{bmatrix}
          \beta_1 \\
          \beta_2 \\
          \beta_3 
        \end{bmatrix}
      \end{equation}
      \begin{equation}
        \begin{bmatrix}
          \beta_1 \\
          \beta_2 \\
          \beta_3 
        \end{bmatrix} = 
        \begin{bmatrix}
          -1.83333 \\
          -1 \\
          -0.16667
        \end{bmatrix}
      \end{equation}
    \item solve for $A^{-1}$
      \begin{equation}
        A^{-1} =
        \beta_0I + \beta_1A + \beta_2A^2 =
        -1.8333I - A - 0.1667A^2 =
        \begin{bmatrix}
          1 & 3 & 0 \\
          -1 & -2.5 & 0 \\
          0 & 0 & 0.33333\\
        \end{bmatrix}
      \end{equation}
      This last step was accomplished with python performing the math
    \end{itemize}
  \item Obtain $e^{At}$ using one of the three mentioned methods in Problem 1 \\
    I am using using the laplace transform method.
    \begin{equation}
\mathscr{L}^{-1}\Big ((sI-A)^{-1}\Big ) = \left[\begin{matrix}\left(4 - 3 e^{t}\right) e^{- 2 t} \theta\left(t\right) & 6 \left(1 - e^{t}\right) e^{- 2 t} \theta\left(t\right) & 0\\2 \left(e^{t} - 1\right) e^{- 2 t} \theta\left(t\right) & \left(4 e^{t} - 3\right) e^{- 2 t} \theta\left(t\right) & 0\\0 & 0 & e^{- 3 t} \theta\left(t\right)\end{matrix}\right]\end{equation}

  \end{enumerate}